proofs/fstar/extraction/Libcrux.Digest.fsti
@@ -12,13 +12,41 @@ val sha3_512_ (payload: t_Slice u8)
 val shake256 (v_LEN: usize) (data: t_Slice u8)
     : Prims.Pure (t_Array u8 v_LEN) Prims.l_True (fun _ -> Prims.l_True)
 
-type t_Shake128State
+type t_Shake128StateX2 =
 
+type t_Shake128StateX3 =
 
-val shake128_absorb_final (st: t_Shake128State) (data: t_Slice u8)
-    : Prims.Pure t_Shake128State Prims.l_True (fun _ -> Prims.l_True)
+type t_Shake128StateX4 =
 
-val shake128_init: Prims.unit -> Prims.Pure t_Shake128State Prims.l_True (fun _ -> Prims.l_True)
+val shake128_absorb_final_x2 (st: t_Shake128StateX2) (data0 data1: t_Slice u8)
+    : Prims.Pure t_Shake128StateX2 Prims.l_True (fun _ -> Prims.l_True)
 
-val shake128_squeeze_nblocks (v_OUTPUT_BYTES: usize) (st: t_Shake128State)
-    : Prims.Pure (t_Shake128State & t_Array u8 v_OUTPUT_BYTES) Prims.l_True (fun _ -> Prims.l_True)
+val shake128_absorb_final_x3 (st: t_Shake128StateX3) (data0 data1 data2: t_Slice u8)
+    : Prims.Pure t_Shake128StateX3 Prims.l_True (fun _ -> Prims.l_True)
+
+val shake128_absorb_final_x4 (st: t_Shake128StateX4) (data0 data1 data2 data3: t_Slice u8)
+    : Prims.Pure t_Shake128StateX4 Prims.l_True (fun _ -> Prims.l_True)
+
+val shake128_init_x2: Prims.unit
+  -> Prims.Pure t_Shake128StateX2 Prims.l_True (fun _ -> Prims.l_True)
+
+val shake128_init_x3: Prims.unit
+  -> Prims.Pure t_Shake128StateX3 Prims.l_True (fun _ -> Prims.l_True)
+
+val shake128_init_x4: Prims.unit
+  -> Prims.Pure t_Shake128StateX4 Prims.l_True (fun _ -> Prims.l_True)
+
+val shake128_squeeze_nblocks_x2 (v_OUTPUT_BYTES: usize) (st: t_Shake128StateX2)
+    : Prims.Pure (t_Shake128StateX2 & t_Array (t_Array u8 v_OUTPUT_BYTES) (sz 2))
+      Prims.l_True
+      (fun _ -> Prims.l_True)
+
+val shake128_squeeze_nblocks_x3 (v_OUTPUT_BYTES: usize) (st: t_Shake128StateX3)
+    : Prims.Pure (t_Shake128StateX3 & t_Array (t_Array u8 v_OUTPUT_BYTES) (sz 3))
+      Prims.l_True
+      (fun _ -> Prims.l_True)
+
+val shake128_squeeze_nblocks_x4 (v_OUTPUT_BYTES: usize) (st: t_Shake128StateX4)
+    : Prims.Pure (t_Shake128StateX4 & t_Array (t_Array u8 v_OUTPUT_BYTES) (sz 4))
+      Prims.l_True
+      (fun _ -> Prims.l_True)
