proofs/fstar/extraction/Libcrux.Kem.Kyber.Ind_cpa.fsti
@@ -52,6 +52,14 @@ val decrypt
       (ciphertext: t_Array u8 v_CIPHERTEXT_SIZE)
     : Prims.Pure (t_Array u8 (sz 32)) Prims.l_True (fun _ -> Prims.l_True)
 
+val encrypt
+      (v_K v_CIPHERTEXT_SIZE v_T_AS_NTT_ENCODED_SIZE v_C1_LEN v_C2_LEN v_U_COMPRESSION_FACTOR v_V_COMPRESSION_FACTOR v_BLOCK_LEN v_ETA1 v_ETA1_RANDOMNESS_SIZE v_ETA2 v_ETA2_RANDOMNESS_SIZE:
+          usize)
+      (public_key: t_Slice u8)
+      (message: t_Array u8 (sz 32))
+      (randomness: t_Slice u8)
+    : Prims.Pure (t_Array u8 v_CIPHERTEXT_SIZE) Prims.l_True (fun _ -> Prims.l_True)
+
 val serialize_secret_key
       (v_K v_OUT_LEN: usize)
       (key: t_Array Libcrux.Kem.Kyber.Arithmetic.t_PolynomialRingElement v_K)
@@ -62,14 +70,6 @@ val serialize_public_key
       (tt_as_ntt: t_Array Libcrux.Kem.Kyber.Arithmetic.t_PolynomialRingElement v_K)
       (seed_for_a: t_Slice u8)
     : Prims.Pure (t_Array u8 v_PUBLIC_KEY_SIZE) Prims.l_True (fun _ -> Prims.l_True)
-
-val encrypt
-      (v_K v_CIPHERTEXT_SIZE v_T_AS_NTT_ENCODED_SIZE v_C1_LEN v_C2_LEN v_U_COMPRESSION_FACTOR v_V_COMPRESSION_FACTOR v_BLOCK_LEN v_ETA1 v_ETA1_RANDOMNESS_SIZE v_ETA2 v_ETA2_RANDOMNESS_SIZE:
-          usize)
-      (public_key: t_Slice u8)
-      (message: t_Array u8 (sz 32))
-      (randomness: t_Slice u8)
-    : Prims.Pure (t_Array u8 v_CIPHERTEXT_SIZE) Prims.l_True (fun _ -> Prims.l_True)
 
 val generate_keypair
       (v_K v_PRIVATE_KEY_SIZE v_PUBLIC_KEY_SIZE v_RANKED_BYTES_PER_RING_ELEMENT v_ETA1 v_ETA1_RANDOMNESS_SIZE:
