proofs/fstar/extraction/Libcrux.Kem.Kyber.fsti
@@ -15,11 +15,6 @@ val serialize_kem_secret_key
       (private_key public_key implicit_rejection_value: t_Slice u8)
     : Prims.Pure (t_Array u8 v_SERIALIZED_KEY_LEN) Prims.l_True (fun _ -> Prims.l_True)
 
-val validate_public_key
-      (v_K v_RANKED_BYTES_PER_RING_ELEMENT v_PUBLIC_KEY_SIZE: usize)
-      (public_key: t_Array u8 v_PUBLIC_KEY_SIZE)
-    : Prims.Pure bool Prims.l_True (fun _ -> Prims.l_True)
-
 val decapsulate
       (v_K v_SECRET_KEY_SIZE v_CPA_SECRET_KEY_SIZE v_PUBLIC_KEY_SIZE v_CIPHERTEXT_SIZE v_T_AS_NTT_ENCODED_SIZE v_C1_SIZE v_C2_SIZE v_VECTOR_U_COMPRESSION_FACTOR v_VECTOR_V_COMPRESSION_FACTOR v_C1_BLOCK_SIZE v_ETA1 v_ETA1_RANDOMNESS_SIZE v_ETA2 v_ETA2_RANDOMNESS_SIZE v_IMPLICIT_REJECTION_HASH_INPUT_SIZE:
           usize)
@@ -35,6 +30,11 @@ val encapsulate
     : Prims.Pure (Libcrux.Kem.Kyber.Types.t_MlKemCiphertext v_CIPHERTEXT_SIZE & t_Array u8 (sz 32))
       Prims.l_True
       (fun _ -> Prims.l_True)
+
+val validate_public_key
+      (v_K v_RANKED_BYTES_PER_RING_ELEMENT v_PUBLIC_KEY_SIZE: usize)
+      (public_key: t_Array u8 v_PUBLIC_KEY_SIZE)
+    : Prims.Pure bool Prims.l_True (fun _ -> Prims.l_True)
 
 val generate_keypair
       (v_K v_CPA_PRIVATE_KEY_SIZE v_PRIVATE_KEY_SIZE v_PUBLIC_KEY_SIZE v_BYTES_PER_RING_ELEMENT v_ETA1 v_ETA1_RANDOMNESS_SIZE:
